checkpoint

pulse/ulib/experimental/Steel.Semantics.fst
@@ -611,356 +611,448 @@ let step_ret (#st:st) (i:nat) #fpre #a #fpost (frame:st.hprop)
          (Ret pp x)
          i
 
-#push-options "--z3rlimit_factor 2 --z3cliopt 'smt.qi.eager_threshold=100'"
-// let elim_lift (#st:st) (r0 r1:st.r) (p:rs_prop r0) (s:st.s)
-//   : Lemma
-//     (requires
-//       st.interp (st.lift r0 p `st.star` r1) s)
-//     (ensures
-//       st.interp (r0 `st.star` r1) s /\
-//       st.interp r0 s /\
-//       st.interp r1 s /\
-//       p s)
-//    = ()
+//#push-options "--z3rlimit_factor 2 --z3cliopt 'smt.qi.eager_threshold=100'"
+let elim_refine (#st:st) (r0 r1:st.hprop) (p:fp_prop r0) (s:st.heap)
+  : Lemma
+    (requires
+      st.interp (st.refine r0 p `st.star` r1) s)
+    (ensures
+      st.interp (r0 `st.star` r1) s /\
+      st.interp r0 s /\
+      st.interp r1 s /\
+      p s)
+   = ()
 
-// let elim_rs_prop (#st:st) (r:st.r) (p:rs_prop r) (s:st.s)
-//   : Lemma
-//     (requires
-//       st.interp r s /\
-//       p s)
-//     (ensures
-// //      st.interp r (fst (st.split r s)) /\
-//       p (fst (st.split r s)))
-//   = ()
+let intro_refine (#st:st) (r0 r1:st.hprop) (p:fp_prop r0) (s:st.heap)
+  : Lemma
+    (requires
+      st.interp (r0 `st.star` r1) s /\
+      p s)
+    (ensures
+      st.interp (st.refine r0 p `st.star` r1) s)
+   = assert (st.interp (st.refine (r0 `st.star` r1) p) s)
 
-#push-options "--z3rlimit_factor 8"
+#push-options "--z3rlimit_factor 4"
+
+let rearrange_action_result
+    (#st:st) (#fpre:st.hprop) #a #fpost (f:action fpre a fpost)
+    (v:a) (s0 s1:st.heap)
+    (q:st.hprop) (r:fp_prop q) (frame:st.hprop)
+  : Pure (action (fpre `st.star` q) a (fun x -> fpost x `st.star` q))
+    (requires
+      action_result f v s0 s1 (st.refine q r `st.star` frame))
+    (ensures fun g ->
+      action_result g v s0 s1 frame)
+  = admit()
+
+
 let rec step (#st:st) (i:nat) #pre #a #post
              (frame:st.hprop)
-             (#wp:wp pre a post)
-             (f:m st a pre post wp)
+             (#wp_:wp pre a post)
+             (f:m st a pre post wp_)
              (k:wp_post a post)
              (state:st.heap)
   : Div (step_result a post frame k)
         (requires
           st.interp (pre `st.star` frame) state /\
           st.interp pre state /\
-          wp k state)
+          wp_ k state)
         (ensures fun _ -> True)
   = match f with
-    | Ret _ _ ->
-       step_ret i frame f k state
+    // | Ret _ _ ->
+    //    step_ret i frame f k state
 
-    | Act _ _ _ _ _  ->
-      step_act i frame f k state
+    // | Act _ _ _ _ _  ->
+    //   step_act i frame f k state
 
-    | Par preL aL postL wpL (Ret _ _)
-          preR aR postR wpR (Ret _ _)
-          post wp_kont kont ->
-      step_par_ret i frame f k state
+    // | Par preL aL postL wpL (Ret _ _)
+    //       preR aR postR wpR (Ret _ _)
+    //       post wp_kont kont ->
+    //   step_par_ret i frame f k state
 
     | Par preL aL postL wpL mL
           preR aR postR wpR mR
           post wp_kont kont ->
 
-      assert (wp == bind_par wpL wpR wp_kont);
+      assert (wp_ == bind_par wpL wpR wp_kont);
       assert (st.interp (preL `st.star` (preR `st.star` frame)) state);
       assert (st.interp (preL `st.star` preR) state);
-
-      let sL, rest0 = st.split preL state in
-      let sR, rest = st.split preR rest0 in
-      assert (as_requires wpL sL);
-      assert (as_requires wpR sR);
-
       assert (as_requires wpL state);
-      assert (as_requires wpR rest0);
-      assert (fst (st.split preR rest0) == fst (st.split preR state));
       assert (as_requires wpR state);
-
-      if bools i
-      then begin
-        calc (st.equals) {
-          preL `st.star` (preR `st.star` frame);
+      calc (st.equals) {
+        preL `st.star` (preR `st.star` frame);
           (st.equals) { }
-          (preL `st.star` preR) `st.star` frame;
+        (preL `st.star` preR) `st.star` frame;
           (st.equals) { }
-          (preR `st.star` preL) `st.star` frame;
+        (preR `st.star` preL) `st.star` frame;
           (st.equals) { }
-          preR `st.star` (preL `st.star` frame);
-        };
-        assert (st.interp ((st.lift preR (as_requires wpR)) `st.star` (preL `st.star` frame)) state);
-        calc (st.equals) {
-          (st.lift preR (as_requires wpR)) `st.star` (preL `st.star` frame);
+        preR `st.star` (preL `st.star` frame);
+      };
+      intro_refine preR (preL `st.star` frame) (as_requires wpR) state;
+      calc (st.equals) {
+        (st.refine preR (as_requires wpR)) `st.star` (preL `st.star` frame);
           (st.equals) { }
-          (st.lift preR (as_requires wpR) `st.star` preL) `st.star` frame;
+        (st.refine preR (as_requires wpR) `st.star` preL) `st.star` frame;
           (st.equals) { }
-          (preL `st.star` st.lift preR (as_requires wpR)) `st.star` frame;
+        (preL `st.star` st.refine preR (as_requires wpR)) `st.star` frame;
           (st.equals) { }
-          preL `st.star` ((st.lift preR (as_requires wpR)) `st.star` frame);
-        };
-        assert (st.interp (preL `st.star` ((st.lift preR (as_requires wpR)) `st.star` frame)) state);
-        let Step preL' wpL' mL' state' j =
+        preL `st.star` ((st.refine preR (as_requires wpR)) `st.star` frame);
+      };
+      let Step fpre b fpost act initial_state v next_state wpL' mL' j =
             //Notice that, inductively, we instantiate the frame extending
             //it to include the precondition of the other side of the par
             step (i + 1)
-                 ((st.lift preR (as_requires wpR)) `st.star` frame)
+                 ((st.refine preR (as_requires wpR)) `st.star` frame)
                  mL
                  (triv_post aL postL)
                  state
-        in
-        assert (as_requires wpL' state');
-        assert (as_requires wpR state');
-        let sL', rest0' = st.split preL' state' in
-        let sR', rest' = st.split preR rest0' in
-        assert (bind_par wpL wpR wp_kont k state ==>
-               bind_par wpL' wpR wp_kont k state')
-               by  (T.norm [delta_only [`%wp_par; `%bind_wp; `%bind_par; `%wp_par_post]];
-               T.dump "A";
-               T.smt());
-        Step (preL' `st.star` preR)
+      in
+      assert (as_requires wpL' next_state);
+      assert (as_requires wpR next_state);
+      let wpL' : wp (fpost v) aL postL = wpL' in
+      let wpR  : wp preR aR postR = wpR in
+      let wp_par
+        : wp (fpost v `st.star` preR) a post
+        = bind_par wpL' wpR wp_kont
+      in
+      let mL' : m st aL (fpost v) postL wpL' = mL' in
+      let next_m
+        : m st a (fpost v `st.star` preR) post wp_par
+        = Par (fpost v) aL postL wpL' mL'
+              preR aR postR wpR mR
+              post wp_kont kont
+      in
+      assume (wp_par k next_state);
+      // assert (st.interp (fpost v `st.star` preR) next_state);
+      // assume (st.interp (fpre `st.star` preR) state);
+      // assert (action_result act v initial_state next_state
+      //        ((st.refine preR (as_requires wpR)) `st.star` frame));
+      assert (action_result act v initial_state next_state (st.refine preR (as_requires wpR) `st.star` frame));
+      let act : action (fpre `st.star` preR) b (fun x -> fpost x `st.star` preR) =
+        rearrange_action_result act v initial_state next_state preR (as_requires wpR) frame
+      in
+      let step =
+        Step (fpre `st.star` preR) b (fun x -> fpost x `st.star` preR) act initial_state v next_state
+             wp_par
+             next_m
+             j
+      in
+      step | _ -> admit()
+
+
+
+      admit()
+
+   | _ -> admit()
+      assume (bind_par wpL' wpR wp_kont k next_state);
+      let step =
+        Step fpre b fpost act initial_state v next_state
              (bind_par wpL' wpR wp_kont)
-             (Par preL' aL postL wpL' mL'
-                  preR  aR postR wpR  mR
-                  post wp_kont kont)
-             state'
-             j
-      end else begin
-        assert (st.interp ((st.lift preL (as_requires wpL)) `st.star` (preR `st.star` frame)) state);
-        calc (st.equals) {
-          (st.lift preL (as_requires wpL)) `st.star` (preR `st.star` frame);
-          (st.equals) { }
-          (st.lift preL (as_requires wpL) `st.star` preR) `st.star` frame;
-          (st.equals) { }
-          (preR `st.star` st.lift preL (as_requires wpL)) `st.star` frame;
-          (st.equals) { }
-          preR `st.star` ((st.lift preL (as_requires wpL)) `st.star` frame);
-        };
-        assert (st.interp (preR `st.star` ((st.lift preL (as_requires wpL)) `st.star` frame)) state);
-        let Step preR' wpR' mR' state' j =
-            //Notice that, inductively, we instantiate the frame extending
-            //it to include the precondition of the other side of the par
-            step (i + 1)
-                 ((st.lift preL (as_requires wpL)) `st.star` frame)
-                 mR
-                 (triv_post aR postR)
-                 state
-        in
-        assert (as_requires wpL state');
-        assert (as_requires wpR' state');
-        let sL', rest0' = st.split preL state' in
-        let sR', rest' = st.split preR' rest0' in
-        assert (bind_par wpL wpR wp_kont k state ==>
-                bind_par wpL wpR' wp_kont k state')
-               by  (T.norm [delta_only [`%wp_par; `%bind_wp; `%bind_par; `%wp_par_post]];
-               T.dump "A";
-               T.smt());
-        let p' = (preL `st.star` preR') in
-        let wp' = bind_par wpL wpR' wp_kont in
-        calc (st.equals) {
-          preR' `st.star` (preL `st.star` frame);
-          (st.equals) { }
-          (preR' `st.star` preL) `st.star` frame;
-          (st.equals) { }
-          (preL `st.star` preR') `st.star` frame;
-        };
-        Step p'
-             wp'
-             (Par preL aL postL wpL mL
-                  preR'  aR postR wpR' mR'
-                  post wp_kont kont)
-             state'
-             j
-      end
+             next_m
+             j in
+      admit();
+      step
+//
+//      admit()
+
+      // let sL, rest0 = st.split preL state in
+      // let sR, rest = st.split preR rest0 in
+      // assert (as_requires wpL sL);
+      // assert (as_requires wpR sR);
+
+      // assert (as_requires wpL state);
+      // assert (as_requires wpR rest0);
+      // assert (fst (st.split preR rest0) == fst (st.split preR state));
+      // assert (as_requires wpR state);
+
+    | _ -> admit()
 
 
-// (**
-// //  * [run i f state]: Top-level driver that repeatedly invokes [step]
-// //  *
-// //  * The type of [run] is the main theorem. It states that it is sound
-// //  * to interpret the indices of `m` as a Hoare triple in a
-// //  * partial-correctness semantics
-// //  *
-// //  *)
-// let rec run (#st:st) (i:nat)
-//             #pre #a #post (#wp:wp pre a post)
-//             (f:m st a pre post wp) (state:st.s)
-//             (k:wp_post a post)
-//   : Div (a & st.s)
-//     (requires
-//       st.interp pre state /\
-//       wp k state)
-//     (ensures fun (x, state') ->
-//       st.interp (post x) state' /\
-//       k x state')
-//   = match f with
-//     | Ret x -> x, state
-//     | _ ->
-//       let Step pre' wp' f' state' j = step i st.emp f k state in
-//       run j f' state' k
+//       if bools i
+//       then begin
+//         calc (st.equals) {
+//           preL `st.star` (preR `st.star` frame);
+//           (st.equals) { }
+//           (preL `st.star` preR) `st.star` frame;
+//           (st.equals) { }
+//           (preR `st.star` preL) `st.star` frame;
+//           (st.equals) { }
+//           preR `st.star` (preL `st.star` frame);
+//         };
+//         assert (st.interp ((st.lift preR (as_requires wpR)) `st.star` (preL `st.star` frame)) state);
+//         calc (st.equals) {
+//           (st.lift preR (as_requires wpR)) `st.star` (preL `st.star` frame);
+//           (st.equals) { }
+//           (st.lift preR (as_requires wpR) `st.star` preL) `st.star` frame;
+//           (st.equals) { }
+//           (preL `st.star` st.lift preR (as_requires wpR)) `st.star` frame;
+//           (st.equals) { }
+//           preL `st.star` ((st.lift preR (as_requires wpR)) `st.star` frame);
+//         };
+//         assert (st.interp (preL `st.star` ((st.lift preR (as_requires wpR)) `st.star` frame)) state);
+//         let Step preL' wpL' mL' state' j =
+//             //Notice that, inductively, we instantiate the frame extending
+//             //it to include the precondition of the other side of the par
+//             step (i + 1)
+//                  ((st.lift preR (as_requires wpR)) `st.star` frame)
+//                  mL
+//                  (triv_post aL postL)
+//                  state
+//         in
+//         assert (as_requires wpL' state');
+//         assert (as_requires wpR state');
+//         let sL', rest0' = st.split preL' state' in
+//         let sR', rest' = st.split preR rest0' in
+//         assert (bind_par wpL wpR wp_kont k state ==>
+//                bind_par wpL' wpR wp_kont k state')
+//                by  (T.norm [delta_only [`%wp_par; `%bind_wp; `%bind_par; `%wp_par_post]];
+//                T.dump "A";
+//                T.smt());
+//         Step (preL' `st.star` preR)
+//              (bind_par wpL' wpR wp_kont)
+//              (Par preL' aL postL wpL' mL'
+//                   preR  aR postR wpR  mR
+//                   post wp_kont kont)
+//              state'
+//              j
+//       end else begin
+//         assert (st.interp ((st.lift preL (as_requires wpL)) `st.star` (preR `st.star` frame)) state);
+//         calc (st.equals) {
+//           (st.lift preL (as_requires wpL)) `st.star` (preR `st.star` frame);
+//           (st.equals) { }
+//           (st.lift preL (as_requires wpL) `st.star` preR) `st.star` frame;
+//           (st.equals) { }
+//           (preR `st.star` st.lift preL (as_requires wpL)) `st.star` frame;
+//           (st.equals) { }
+//           preR `st.star` ((st.lift preL (as_requires wpL)) `st.star` frame);
+//         };
+//         assert (st.interp (preR `st.star` ((st.lift preL (as_requires wpL)) `st.star` frame)) state);
+//         let Step preR' wpR' mR' state' j =
+//             //Notice that, inductively, we instantiate the frame extending
+//             //it to include the precondition of the other side of the par
+//             step (i + 1)
+//                  ((st.lift preL (as_requires wpL)) `st.star` frame)
+//                  mR
+//                  (triv_post aR postR)
+//                  state
+//         in
+//         assert (as_requires wpL state');
+//         assert (as_requires wpR' state');
+//         let sL', rest0' = st.split preL state' in
+//         let sR', rest' = st.split preR' rest0' in
+//         assert (bind_par wpL wpR wp_kont k state ==>
+//                 bind_par wpL wpR' wp_kont k state')
+//                by  (T.norm [delta_only [`%wp_par; `%bind_wp; `%bind_par; `%wp_par_post]];
+//                T.dump "A";
+//                T.smt());
+//         let p' = (preL `st.star` preR') in
+//         let wp' = bind_par wpL wpR' wp_kont in
+//         calc (st.equals) {
+//           preR' `st.star` (preL `st.star` frame);
+//           (st.equals) { }
+//           (preR' `st.star` preL) `st.star` frame;
+//           (st.equals) { }
+//           (preL `st.star` preR') `st.star` frame;
+//         };
+//         Step p'
+//              wp'
+//              (Par preL aL postL wpL mL
+//                   preR'  aR postR wpR' mR'
+//                   post wp_kont kont)
+//              state'
+//              j
+//       end
 
 
-// ////////////////////////////////////////////////////////////////////////////////
-// //The rest of this module shows how these semantics can be packaged up as an
-// //effect in F*
-// ////////////////////////////////////////////////////////////////////////////////
-
-// (** [eff a pre post] : The representation-type for a layered effect
-// //  *
-// //  *   - Note, we'll probably have to add a thunk to make it work with
-// //  *     the current implementation but that's a detail
-// //  *)
-// let eff (#st:st) a
-//         (expects:st.r)
-//         (provides: a -> st.r)
-//         (wp:wp expects a provides)
-//   = m st a expects provides wp
-
-// /// eff is a monad: we give a return and bind for it, though we don't
-// /// prove the monad laws
-
-
-// (** [return]: easy, just use Ret *)
-// let return (#st:st) #a (x:a) (post:a -> st.r)
-//   : eff a (post x) post (return_wp x post)
-//   = Ret x
-
-// let eta2 #a #b #c (f:a -> b -> c) : Lemma ((fun x y -> f x y) == f) = ()
-
-// (**
-// //  * [bind]: sequential composition works by pushing `g` into the continuation
-// //  * at each node, finally applying it at the terminal `Ret`
-// //  *)
-// let rec bind (#st:st) #a #b (#p:st.r) (#q:a -> st.r) (#r:b -> st.r)
-//              (#wp_f: wp p a q) (f:eff a p q wp_f)
-//              (#wp_g: (x:a -> wp (q x) b r)) (g: (x:a -> eff b (q x) r (wp_g x)))
-//   : Dv (eff b p r (bind_wp wp_f wp_g))
-//   = match f with
-//     | Ret x ->
-//       assert (p == q x);
-//       assert (wp_f == return_wp x q);
-//       assert (eq2 #(wp_post b r -> rs (q x) -> prop) (bind_wp (return_wp x q) wp_g) (wp_g x))
-//         by (T.norm [delta_only [`%bind_wp; `%return_wp]];
-//             T.dump "A";
-//             T.mapply (`eta2));
-//       g x
-
-//     | Act #_ #a' f #post_h #wp_h h ->
-//       assert (wp_f == bind_action f wp_h);
-//       let g' (x:_) : Dv (eff b (f.post x) r (bind_wp (wp_h x) wp_g))
-//         = bind #st #a' #b (h x) g
-//       in
-//       let res : eff b p r (bind_action f (fun x -> bind_wp (wp_h x) wp_g)) = Act f g' in
-//       calc (==) {
-//         bind_action f (fun x -> bind_wp (wp_h x) wp_g);
-//           == {}
-//         bind_wp (wp_action f) (fun x -> bind_wp (wp_h x) wp_g);
-//           == { admit() (* assoc *) }
-//         bind_wp (bind_wp (wp_action f) (fun x -> wp_h x)) wp_g;
-//           == { }
-//         bind_wp wp_f wp_g;
-//       };
-//       res
-
-//     | Par preL aL postL wpL mL
-//           preR aR postR wpR mR
-//           post wp_kont kont ->
-//       let kont x0 x1 : Dv (eff b (postL x0 `st.star` postR x1) r (bind_wp (wp_kont x0 x1) wp_g)) = bind (kont x0 x1) g in
-//       let res : m st b (st.star preL preR) r (bind_par wpL wpR (fun x0 x1 -> (bind_wp (wp_kont x0 x1) wp_g))) =
-//           Par preL aL postL wpL mL
-//                     preR aR postR wpR mR
-//                     r (fun x0 x1 -> (bind_wp (wp_kont x0 x1) wp_g)) kont in
-//       calc (==) {
-//         (bind_par wpL wpR (fun x0 x1 -> (bind_wp (wp_kont x0 x1) wp_g)));
-//         == { _ by (T.dump "A"; T.norm [delta_only [`%bind_par]]; T.dump "B"; T.trefl()) }
-//         bind_wp (wp_par wpL wpR) (fun (x0, x1) -> (bind_wp (wp_kont x0 x1) wp_g));
-//         == { admit () (* assoc *) }
-//         bind_wp (bind_wp (wp_par wpL wpR) (fun (x0, x1) -> wp_kont x0 x1)) wp_g;
-//         == {}
-//         (bind_wp (bind_par wpL wpR wp_kont) wp_g);
-//       };
-//       res
+// // (**
+// // //  * [run i f state]: Top-level driver that repeatedly invokes [step]
+// // //  *
+// // //  * The type of [run] is the main theorem. It states that it is sound
+// // //  * to interpret the indices of `m` as a Hoare triple in a
+// // //  * partial-correctness semantics
+// // //  *
+// // //  *)
+// // let rec run (#st:st) (i:nat)
+// //             #pre #a #post (#wp:wp pre a post)
+// //             (f:m st a pre post wp) (state:st.s)
+// //             (k:wp_post a post)
+// //   : Div (a & st.s)
+// //     (requires
+// //       st.interp pre state /\
+// //       wp k state)
+// //     (ensures fun (x, state') ->
+// //       st.interp (post x) state' /\
+// //       k x state')
+// //   = match f with
+// //     | Ret x -> x, state
+// //     | _ ->
+// //       let Step pre' wp' f' state' j = step i st.emp f k state in
+// //       run j f' state' k
 
 
-// // // // // (**
-// // // // //  * [par]: Parallel composition
-// // // // //  * Works by just using the `Par` node and `Ret` as its continuation
-// // // // //  **)
-// // // // // let par #s (#c:comm_monoid s)
-// // // // //         #a0 #p0 #q0 (m0:eff a0 p0 q0)
-// // // // //         #a1 #p1 #q1 (m1:eff a1 p1 q1)
-// // // // //  : eff (a0 & a1) (p0 `c.star` p1) (fun (x0, x1) -> q0 x0 `c.star` q1 x1)
-// // // // //  = Par p0 q0 m0
-// // // // //        p1 q1 m1
-// // // // //        #_ #(fun (x0, x1) -> c.star (q0 x0) (q1 x1)) (fun x0 x1 -> Ret (x0, x1))
+// // ////////////////////////////////////////////////////////////////////////////////
+// // //The rest of this module shows how these semantics can be packaged up as an
+// // //effect in F*
+// // ////////////////////////////////////////////////////////////////////////////////
+
+// // (** [eff a pre post] : The representation-type for a layered effect
+// // //  *
+// // //  *   - Note, we'll probably have to add a thunk to make it work with
+// // //  *     the current implementation but that's a detail
+// // //  *)
+// // let eff (#st:st) a
+// //         (expects:st.r)
+// //         (provides: a -> st.r)
+// //         (wp:wp expects a provides)
+// //   = m st a expects provides wp
+
+// // /// eff is a monad: we give a return and bind for it, though we don't
+// // /// prove the monad laws
 
 
-// // // // // /// Now for an instantiation of the state with a heap
-// // // // // /// just to demonstrate how that would go
+// // (** [return]: easy, just use Ret *)
+// // let return (#st:st) #a (x:a) (post:a -> st.r)
+// //   : eff a (post x) post (return_wp x post)
+// //   = Ret x
 
-// // // // // /// Heaps are usually in a universe higher than the values they store
-// // // // // /// Pick it in universe 1
-// // // // // assume val heap : Type u#1
+// // let eta2 #a #b #c (f:a -> b -> c) : Lemma ((fun x y -> f x y) == f) = ()
 
-// // // // // /// Assume some monoid of heap assertions
-// // // // // assume val hm : comm_monoid heap
+// // (**
+// // //  * [bind]: sequential composition works by pushing `g` into the continuation
+// // //  * at each node, finally applying it at the terminal `Ret`
+// // //  *)
+// // let rec bind (#st:st) #a #b (#p:st.r) (#q:a -> st.r) (#r:b -> st.r)
+// //              (#wp_f: wp p a q) (f:eff a p q wp_f)
+// //              (#wp_g: (x:a -> wp (q x) b r)) (g: (x:a -> eff b (q x) r (wp_g x)))
+// //   : Dv (eff b p r (bind_wp wp_f wp_g))
+// //   = match f with
+// //     | Ret x ->
+// //       assert (p == q x);
+// //       assert (wp_f == return_wp x q);
+// //       assert (eq2 #(wp_post b r -> rs (q x) -> prop) (bind_wp (return_wp x q) wp_g) (wp_g x))
+// //         by (T.norm [delta_only [`%bind_wp; `%return_wp]];
+// //             T.dump "A";
+// //             T.mapply (`eta2));
+// //       g x
 
-// // // // // /// For this demo, we'll also assume that this assertions are affine
-// // // // // ///  i.e., it's ok to forget some properties of the heap
-// // // // // assume val hm_affine (r0 r1:hm.r) (h:heap)
-// // // // //   : Lemma (hm.interp (r0 `hm.star` r1) h ==>
-// // // // //            hm.interp r0 h)
+// //     | Act #_ #a' f #post_h #wp_h h ->
+// //       assert (wp_f == bind_action f wp_h);
+// //       let g' (x:_) : Dv (eff b (f.post x) r (bind_wp (wp_h x) wp_g))
+// //         = bind #st #a' #b (h x) g
+// //       in
+// //       let res : eff b p r (bind_action f (fun x -> bind_wp (wp_h x) wp_g)) = Act f g' in
+// //       calc (==) {
+// //         bind_action f (fun x -> bind_wp (wp_h x) wp_g);
+// //           == {}
+// //         bind_wp (wp_action f) (fun x -> bind_wp (wp_h x) wp_g);
+// //           == { admit() (* assoc *) }
+// //         bind_wp (bind_wp (wp_action f) (fun x -> wp_h x)) wp_g;
+// //           == { }
+// //         bind_wp wp_f wp_g;
+// //       };
+// //       res
 
-// // // // // /// Here's a ref type
-// // // // // assume val ref : Type u#0 -> Type u#0
+// //     | Par preL aL postL wpL mL
+// //           preR aR postR wpR mR
+// //           post wp_kont kont ->
+// //       let kont x0 x1 : Dv (eff b (postL x0 `st.star` postR x1) r (bind_wp (wp_kont x0 x1) wp_g)) = bind (kont x0 x1) g in
+// //       let res : m st b (st.star preL preR) r (bind_par wpL wpR (fun x0 x1 -> (bind_wp (wp_kont x0 x1) wp_g))) =
+// //           Par preL aL postL wpL mL
+// //                     preR aR postR wpR mR
+// //                     r (fun x0 x1 -> (bind_wp (wp_kont x0 x1) wp_g)) kont in
+// //       calc (==) {
+// //         (bind_par wpL wpR (fun x0 x1 -> (bind_wp (wp_kont x0 x1) wp_g)));
+// //         == { _ by (T.dump "A"; T.norm [delta_only [`%bind_par]]; T.dump "B"; T.trefl()) }
+// //         bind_wp (wp_par wpL wpR) (fun (x0, x1) -> (bind_wp (wp_kont x0 x1) wp_g));
+// //         == { admit () (* assoc *) }
+// //         bind_wp (bind_wp (wp_par wpL wpR) (fun (x0, x1) -> wp_kont x0 x1)) wp_g;
+// //         == {}
+// //         (bind_wp (bind_par wpL wpR wp_kont) wp_g);
+// //       };
+// //       res
 
-// // // // // /// And two atomic heap assertions
-// // // // // assume val ptr_live (r:ref 'a) : hm.r
-// // // // // assume val pts_to (r:ref 'a) (x:'a) : hm.r
 
-// // // // // /// sel: Selected a reference from a heap, when that ref is live
-// // // // // assume val sel (x:ref 'a) (h:heap{hm.interp (ptr_live x) h})
-// // // // //   : Tot 'a
-// // // // // /// this tells us that sel is frameable
-// // // // // assume val sel_ok (x:ref 'a) (h:heap) (frame:hm.r)
-// // // // //   : Lemma (hm.interp (ptr_live x `hm.star` frame) h ==>
-// // // // //            (hm_affine (ptr_live x) frame h;
-// // // // //             let v = sel x h in
-// // // // //             hm.interp (pts_to x v `hm.star` frame) h))
+// // // // // // (**
+// // // // // //  * [par]: Parallel composition
+// // // // // //  * Works by just using the `Par` node and `Ret` as its continuation
+// // // // // //  **)
+// // // // // // let par #s (#c:comm_monoid s)
+// // // // // //         #a0 #p0 #q0 (m0:eff a0 p0 q0)
+// // // // // //         #a1 #p1 #q1 (m1:eff a1 p1 q1)
+// // // // // //  : eff (a0 & a1) (p0 `c.star` p1) (fun (x0, x1) -> q0 x0 `c.star` q1 x1)
+// // // // // //  = Par p0 q0 m0
+// // // // // //        p1 q1 m1
+// // // // // //        #_ #(fun (x0, x1) -> c.star (q0 x0) (q1 x1)) (fun x0 x1 -> Ret (x0, x1))
 
 
-// // // // // /// upd: updates a heap at a given reference, when the heap contains it
-// // // // // assume val upd (x:ref 'a) (v:'a) (h:heap{hm.interp (ptr_live x) h})
-// // // // //   : Tot heap
-// // // // // /// and upd is frameable too
-// // // // // assume val upd_ok (x:ref 'a) (v:'a) (h:heap) (frame:hm.r)
-// // // // //   : Lemma (hm.interp (ptr_live x `hm.star` frame) h ==>
-// // // // //            (hm_affine (ptr_live x) frame h;
-// // // // //             let h' = upd x v h in
-// // // // //             hm.interp (pts_to x v `hm.star` frame) h'))
+// // // // // // /// Now for an instantiation of the state with a heap
+// // // // // // /// just to demonstrate how that would go
 
-// // // // // /// Here's a sample action for dereference
-// // // // // let (!) (x:ref 'a)
-// // // // //   : eff 'a (ptr_live x) (fun v -> pts_to x v)
-// // // // //   = let act : action hm 'a =
-// // // // //     {
-// // // // //       pre = ptr_live x;
-// // // // //       post = pts_to x;
-// // // // //       sem = (fun frame h0 ->
-// // // // //         hm_affine (ptr_live x) frame h0;
-// // // // //         sel_ok x h0 frame;
-// // // // //         (| sel x h0, h0 |))
-// // // // //     } in
-// // // // //     Act act Ret
+// // // // // // /// Heaps are usually in a universe higher than the values they store
+// // // // // // /// Pick it in universe 1
+// // // // // // assume val heap : Type u#1
 
-// // // // // /// And a sample action for assignment
-// // // // // let (:=) (x:ref 'a) (v:'a)
-// // // // //   : eff unit (ptr_live x) (fun _ -> pts_to x v)
-// // // // //   = let act : action hm unit =
-// // // // //     {
-// // // // //       pre = ptr_live x;
-// // // // //       post = (fun _ -> pts_to x v);
-// // // // //       sem = (fun frame h0 ->
-// // // // //         hm_affine (ptr_live x) frame h0;
-// // // // //         upd_ok x v h0 frame;
-// // // // //         (| (), upd x v h0 |))
-// // // // //     } in
-// // // // //     Act act Ret
+// // // // // // /// Assume some monoid of heap assertions
+// // // // // // assume val hm : comm_monoid heap
+
+// // // // // // /// For this demo, we'll also assume that this assertions are affine
+// // // // // // ///  i.e., it's ok to forget some properties of the heap
+// // // // // // assume val hm_affine (r0 r1:hm.r) (h:heap)
+// // // // // //   : Lemma (hm.interp (r0 `hm.star` r1) h ==>
+// // // // // //            hm.interp r0 h)
+
+// // // // // // /// Here's a ref type
+// // // // // // assume val ref : Type u#0 -> Type u#0
+
+// // // // // // /// And two atomic heap assertions
+// // // // // // assume val ptr_live (r:ref 'a) : hm.r
+// // // // // // assume val pts_to (r:ref 'a) (x:'a) : hm.r
+
+// // // // // // /// sel: Selected a reference from a heap, when that ref is live
+// // // // // // assume val sel (x:ref 'a) (h:heap{hm.interp (ptr_live x) h})
+// // // // // //   : Tot 'a
+// // // // // // /// this tells us that sel is frameable
+// // // // // // assume val sel_ok (x:ref 'a) (h:heap) (frame:hm.r)
+// // // // // //   : Lemma (hm.interp (ptr_live x `hm.star` frame) h ==>
+// // // // // //            (hm_affine (ptr_live x) frame h;
+// // // // // //             let v = sel x h in
+// // // // // //             hm.interp (pts_to x v `hm.star` frame) h))
+
+
+// // // // // // /// upd: updates a heap at a given reference, when the heap contains it
+// // // // // // assume val upd (x:ref 'a) (v:'a) (h:heap{hm.interp (ptr_live x) h})
+// // // // // //   : Tot heap
+// // // // // // /// and upd is frameable too
+// // // // // // assume val upd_ok (x:ref 'a) (v:'a) (h:heap) (frame:hm.r)
+// // // // // //   : Lemma (hm.interp (ptr_live x `hm.star` frame) h ==>
+// // // // // //            (hm_affine (ptr_live x) frame h;
+// // // // // //             let h' = upd x v h in
+// // // // // //             hm.interp (pts_to x v `hm.star` frame) h'))
+
+// // // // // // /// Here's a sample action for dereference
+// // // // // // let (!) (x:ref 'a)
+// // // // // //   : eff 'a (ptr_live x) (fun v -> pts_to x v)
+// // // // // //   = let act : action hm 'a =
+// // // // // //     {
+// // // // // //       pre = ptr_live x;
+// // // // // //       post = pts_to x;
+// // // // // //       sem = (fun frame h0 ->
+// // // // // //         hm_affine (ptr_live x) frame h0;
+// // // // // //         sel_ok x h0 frame;
+// // // // // //         (| sel x h0, h0 |))
+// // // // // //     } in
+// // // // // //     Act act Ret
+
+// // // // // // /// And a sample action for assignment
+// // // // // // let (:=) (x:ref 'a) (v:'a)
+// // // // // //   : eff unit (ptr_live x) (fun _ -> pts_to x v)
+// // // // // //   = let act : action hm unit =
+// // // // // //     {
+// // // // // //       pre = ptr_live x;
+// // // // // //       post = (fun _ -> pts_to x v);
+// // // // // //       sem = (fun frame h0 ->
+// // // // // //         hm_affine (ptr_live x) frame h0;
+// // // // // //         upd_ok x v h0 frame;
+// // // // // //         (| (), upd x v h0 |))
+// // // // // //     } in
+// // // // // //     Act act Ret
